



# MAA304: Asymptotic Statistics

Jagan Koipallil

Homework 1

October 4, 2025

**Exercise 1.** Suppose that  $R$  and  $U$  are independent continuous random variables where  $U$  has a Uniform distribution on  $[0, 1]$  and  $R$  has the density function

$$f_R(x) = x \exp(-x^2/2) \quad \text{for } x \geq 0.$$

1. Show that  $R^2$  has an Exponential distribution.
2. Define  $X = R \cos(2\pi U)$  and  $Y = R \sin(2\pi U)$ . Show that  $X$  and  $Y$  are independent standard Normal random variables.
3. Suggest a method for generating Normal random variables based on the results in parts (a) and (b).

**Solution.** 1. Let  $Z = R^2$ . Then  $R = \sqrt{Z}$ , and  $\frac{dR}{dZ} = \frac{1}{2\sqrt{Z}}$ . The density of  $R$  is

$$f_R(x) = x e^{-x^2/2}, \quad x \geq 0.$$

By the transformation formula:

$$f_Z(z) = f_R(\sqrt{z}) \cdot \left| \frac{dR}{dz} \right| = (\sqrt{z} e^{-z/2}) \cdot \frac{1}{2\sqrt{z}} = \frac{1}{2} e^{-z/2}, \quad z \geq 0.$$

This is the density of an Exponential distribution with rate parameter  $\lambda = \frac{1}{2}$  (or mean 2). Thus,

$$\boxed{R^2 \sim \text{Exp}(1/2)}$$

2. Let  $\Theta = 2\pi U$ , so  $\Theta \sim \text{Uniform}(0, 2\pi)$ . The joint density of  $(R, \Theta)$  is

$$f_{R,\Theta}(r, \theta) = f_R(r) \cdot \frac{1}{2\pi} = \frac{1}{2\pi} \cdot r e^{-r^2/2}, \quad r \geq 0, \theta \in [0, 2\pi).$$

Transform  $(R, \Theta) \rightarrow (X, Y)$  by  $X = R \cos \Theta$ ,  $Y = R \sin \Theta$ .

The Jacobian of the transformation  $(r, \theta) \rightarrow (x, y)$  is:

$$J = \begin{vmatrix} \frac{\partial x}{\partial r} & \frac{\partial x}{\partial \theta} \\ \frac{\partial y}{\partial r} & \frac{\partial y}{\partial \theta} \end{vmatrix} = \begin{vmatrix} \cos \theta & -r \sin \theta \\ \sin \theta & r \cos \theta \end{vmatrix} = r \cos^2 \theta + r \sin^2 \theta = r$$

Thus, the Jacobian determinant is  $|J| = r$ , and since  $dx dy = r dr d\theta$ :

$$f_{X,Y}(x, y) = \frac{f_{R,\Theta}(r, \theta)}{r} = \frac{1}{2\pi} e^{-r^2/2}, \quad \text{where } r^2 = x^2 + y^2.$$

So,

$$f_{X,Y}(x, y) = \frac{1}{2\pi} e^{-(x^2+y^2)/2} = \left( \frac{1}{\sqrt{2\pi}} e^{-x^2/2} \right) \left( \frac{1}{\sqrt{2\pi}} e^{-y^2/2} \right).$$

Therefore,

$$\boxed{X \text{ and } Y \text{ are independent } N(0, 1)}$$

3. Generate  $U_1, U_2$  independent Uniform(0, 1). Let  $R^2 = -2 \ln U_1$ , so  $R = \sqrt{-2 \ln U_1}$ . Let  $\Theta = 2\pi U_2$ . Then set

$$X = R \cos \Theta, \quad Y = R \sin \Theta.$$

Then  $X$  and  $Y$  are i.i.d.  $N(0, 1)$ . This is the **Box–Muller method**:

$$\boxed{X = \sqrt{-2 \ln U_1} \cos(2\pi U_2), \quad Y = \sqrt{-2 \ln U_1} \sin(2\pi U_2)}$$

**Exercise 2.** Suppose that  $X_1, \dots, X_n$  are i.i.d. continuous random variables with distribution function  $F(x)$  and density function  $f(x)$ ; let  $X_{(1)} < X_{(2)} < \dots < X_{(n)}$  be the order statistics.

1. Show that the distribution function of  $X_{(k)}$  is

$$G_k(x) = \sum_{j=k}^n \binom{n}{j} F(x)^j (1 - F(x))^{n-j}.$$

2. Show that the density function of  $X_{(k)}$  is

$$g_k(x) = \frac{n!}{(n-k)!(k-1)!} F(x)^{k-1} (1 - F(x))^{n-k} f(x).$$

**Solution.** 1. Let  $Y_i = \mathbb{I}(X_i \leq x)$ , and  $S = \sum_{i=1}^n Y_i$ . Then  $Y_i$  are i.i.d. Bernoulli( $F(x)$ ), so  $S \sim \text{Binomial}(n, F(x))$ . The event  $\{X_{(k)} \leq x\}$  means at least  $k$  of the  $X_i$  are  $\leq x$ , i.e.,  $S \geq k$ . Thus,

$$\mathbb{P}(X_{(k)} \leq x) = \mathbb{P}(S \geq k) = \sum_{j=k}^n \binom{n}{j} F(x)^j (1 - F(x))^{n-j}.$$

$$G_k(x) = \sum_{j=k}^n \binom{n}{j} F(x)^j (1 - F(x))^{n-j}$$

2. Differentiate  $G_k(x)$  term by term:

$$G_k(x) = \sum_{j=k}^n \binom{n}{j} F(x)^j (1 - F(x))^{n-j}.$$

For a fixed  $j$ , the derivative of  $F^j(1 - F)^{n-j}$  is

$$jF^{j-1}f \cdot (1-F)^{n-j} + F^j \cdot (n-j)(1-F)^{n-j-1}(-f) = f[jF^{j-1}(1-F)^{n-j} - (n-j)F^j(1-F)^{n-j-1}].$$

So,

$$g_k(x) = f(x) \sum_{j=k}^n \binom{n}{j} [jF^{j-1}(1-F)^{n-j} - (n-j)F^j(1-F)^{n-j-1}].$$

Note:  $\binom{n}{j}j = n\binom{n-1}{j-1}$ , and  $\binom{n}{j}(n-j) = n\binom{n-1}{j}$ . Thus, the first sum becomes

$$\sum_{j=k}^n n\binom{n-1}{j-1} F^{j-1}(1-F)^{n-j}.$$

Let  $m = j - 1$ , then  $m$  runs from  $k - 1$  to  $n - 1$ :

$$n \sum_{m=k-1}^{n-1} \binom{n-1}{m} F^m (1-F)^{n-1-m}.$$

The second sum becomes

$$\sum_{j=k}^n n\binom{n-1}{j} F^j (1-F)^{n-j-1} = n \sum_{m=k}^n \binom{n-1}{m} F^m (1-F)^{n-1-m}.$$

Subtracting the second from the first gives a telescoping sum, leaving only the  $m = k - 1$  term:

$$n\binom{n-1}{k-1} F^{k-1} (1-F)^{n-k}.$$

Therefore,

$$g_k(x) = f(x) \cdot n \binom{n-1}{k-1} F(x)^{k-1} (1-F(x))^{n-k} = \frac{n!}{(k-1)!(n-k)!} F(x)^{k-1} (1-F(x))^{n-k} f(x).$$

$$g_k(x) = \frac{n!}{(n-k)!(k-1)!} F(x)^{k-1} (1-F(x))^{n-k} f(x)$$

**Exercise 3.** Suppose that  $X_1, \dots, X_n$  are i.i.d. Exponential random variables with parameter  $\lambda$ . Let  $X_{(1)} < \dots < X_{(n)}$  be the order statistics and define

$$\begin{aligned} Y_1 &= nX_{(1)} \\ Y_2 &= (n-1)(X_{(2)} - X_{(1)}) \\ Y_3 &= (n-2)(X_{(3)} - X_{(2)}) \\ &\vdots \\ Y_n &= X_{(n)} - X_{(n-1)}. \end{aligned}$$

Show that  $Y_1, \dots, Y_n$  are i.i.d. Exponential random variables with parameter  $\lambda$ .

**Solution.** The joint density of the order statistics  $X_{(1)}, \dots, X_{(n)}$  for i.i.d. Exponential( $\lambda$ ) is

$$f_{X_{(1)}, \dots, X_{(n)}}(x_1, \dots, x_n) = n! \lambda^n e^{-\lambda(x_1 + \dots + x_n)}, \quad 0 \leq x_1 \leq \dots \leq x_n.$$

Define the transformation:

$$\begin{aligned} y_1 &= nx_1 \\ y_2 &= (n-1)(x_2 - x_1) \\ y_3 &= (n-2)(x_3 - x_2) \\ &\vdots \\ y_n &= x_n - x_{n-1}. \end{aligned}$$

Inverting:

$$\begin{aligned} x_1 &= \frac{y_1}{n} \\ x_2 &= x_1 + \frac{y_2}{n-1} = \frac{y_1}{n} + \frac{y_2}{n-1} \\ x_3 &= x_2 + \frac{y_3}{n-2} = \frac{y_1}{n} + \frac{y_2}{n-1} + \frac{y_3}{n-2} \\ &\vdots \\ x_k &= \sum_{i=1}^k \frac{y_i}{n-i+1}. \end{aligned}$$

The Jacobian matrix  $\frac{\partial x}{\partial y}$  is lower triangular:

$$\frac{\partial x}{\partial y} = \begin{pmatrix} \frac{1}{n} & 0 & 0 & \dots & 0 \\ \frac{1}{n} & \frac{1}{n-1} & 0 & \dots & 0 \\ \frac{1}{n} & \frac{1}{n-1} & \frac{1}{n-2} & \dots & 0 \\ \vdots & \vdots & \vdots & \ddots & \vdots \\ \frac{1}{n} & \frac{1}{n-1} & \frac{1}{n-2} & \dots & 1 \end{pmatrix}$$

The determinant is the product of the diagonal entries:

$$\left| \frac{\partial x}{\partial y} \right| = \frac{1}{n} \cdot \frac{1}{n-1} \cdots \frac{1}{1} = \frac{1}{n!}.$$

Now we compute  $\sum_{i=1}^n x_i$ :

$$\sum_{i=1}^n x_i = \sum_{i=1}^n \sum_{j=1}^i \frac{y_j}{n-j+1}.$$

Changing the order of summation (for each  $j$ , sum over all  $i \geq j$ ):

$$= \sum_{j=1}^n \sum_{i=j}^n \frac{y_j}{n-j+1} = \sum_{j=1}^n \frac{y_j}{n-j+1} \sum_{i=j}^n 1 = \sum_{j=1}^n \frac{y_j}{n-j+1} \cdot (n-j+1) = \sum_{j=1}^n y_j.$$

Thus, the joint density of  $Y_1, \dots, Y_n$  is

$$f_Y(y_1, \dots, y_n) = n! \lambda^n e^{-\lambda \sum y_i} \cdot \frac{1}{n!} = \lambda^n e^{-\lambda \sum_{i=1}^n y_i}, \quad y_i \geq 0.$$

This factors as  $\prod_{i=1}^n [\lambda e^{-\lambda y_i}]$ .

Therefore,

$$\boxed{Y_1, \dots, Y_n \text{ are i.i.d. Exponential}(\lambda)}$$

**Exercise 4.** Let  $(X, Y)$  be a 2-dimensional Gaussian vector with probability density

$$f(x, y) = \frac{1}{2\pi(1-\rho^2)^{1/2}} \exp \left\{ -\frac{1}{2(1-\rho^2)} (x^2 - 2\rho xy + y^2) \right\}$$

where  $|\rho| < 1$ .

1. Show that  $X$  and  $(Y - \rho X) / (1 - \rho^2)^{1/2}$  are independent Gaussian random variables with mean 0 and variance 1.

2. Show that

$$\begin{aligned} \mathbb{P}(X > 0, Y > 0) &= \mathbb{P}\left(X > 0, \rho X + Z(1 - \rho^2)^{1/2} > 0\right) \\ &= \mathbb{P}\left(X > 0, Z > -\frac{\rho}{(1 - \rho^2)^{1/2}} X\right). \end{aligned}$$

3. Compute

$$\mathbb{P}(X > 0, Y > 0) = \frac{1}{4} + \frac{1}{2\pi} \sin^{-1}(\rho).$$

**Solution.** 1. Complete the square in the exponent:

$$x^2 - 2\rho xy + y^2 = (y - \rho x)^2 + x^2(1 - \rho^2).$$

So the exponent becomes

$$-\frac{(y - \rho x)^2}{2(1 - \rho^2)} - \frac{x^2}{2}.$$

Thus,

$$f(x, y) = \frac{1}{\sqrt{2\pi}} e^{-x^2/2} \cdot \frac{1}{\sqrt{2\pi}\sqrt{1-\rho^2}} \exp \left[ -\frac{(y - \rho x)^2}{2(1 - \rho^2)} \right].$$

Let  $Z = \frac{Y - \rho X}{\sqrt{1 - \rho^2}}$ . Given  $X = x$ ,  $Y \sim N(\rho x, 1 - \rho^2)$ , so  $Z \sim N(0, 1)$  and is independent of  $X$  because the conditional density of  $Z$  given  $X$  is standard normal.

Therefore,

$$X \text{ and } Z = \frac{Y - \rho X}{\sqrt{1 - \rho^2}} \text{ are independent } N(0, 1)$$

2. Since  $Y = \rho X + \sqrt{1 - \rho^2}Z$ , the condition  $Y > 0$  is equivalent to

$$Z > -\frac{\rho X}{\sqrt{1 - \rho^2}}.$$

Thus,

$$\mathbb{P}(X > 0, Y > 0) = \mathbb{P}\left(X > 0, Z > -\frac{\rho X}{\sqrt{1 - \rho^2}}\right).$$

3. Let  $(X, Z)$  be i.i.d.  $N(0, 1)$ . Transform to polar coordinates:  $X = R \cos \Phi$ ,  $Z = R \sin \Phi$ , with  $R > 0$ ,  $\Phi \in [0, 2\pi)$ . The condition  $X > 0$  means  $\cos \Phi > 0$ , i.e.,  $\Phi \in (-\pi/2, \pi/2)$ . The condition  $Z > -\frac{\rho}{\sqrt{1 - \rho^2}}X$  becomes

$$R \sin \Phi > -R \cos \Phi \cdot \frac{\rho}{\sqrt{1 - \rho^2}} \implies \tan \Phi > -\frac{\rho}{\sqrt{1 - \rho^2}}.$$

Let  $\theta = \arcsin(\rho)$ , so  $\sin \theta = \rho$ ,  $\cos \theta = \sqrt{1 - \rho^2}$ , and  $\tan \theta = \frac{\rho}{\sqrt{1 - \rho^2}}$ . Then the inequality becomes  $\Phi > -\theta$ . Within  $(-\pi/2, \pi/2)$ , this means  $\Phi \in (-\theta, \pi/2)$ . The length of this interval is  $\pi/2 + \theta$ . By circular symmetry of the bivariate standard normal, the probability is

$$\frac{\pi/2 + \theta}{2\pi} = \frac{1}{4} + \frac{\theta}{2\pi}.$$

Since  $\theta = \arcsin(\rho)$ , we have:

$$\mathbb{P}(X > 0, Y > 0) = \frac{1}{4} + \frac{1}{2\pi} \arcsin(\rho)$$